compiler/wasm/README.md
@@ -18,6 +18,11 @@ Compilation from stackLang to wasmLang
 
 [wasm2LangScript.sml](wasm2LangScript.sml):
 CWasm AST modelling Wasm 2.0 (+ tail calls)
+Present here are
+  + control flow instructions
+  + all numeric (stack) instructions
+  + all vector (stack) instructions
+  + all (incl num&vec) memory operations -- factored into their own datatype
 Imprecisions:
   HOL lists encode Wasm vectors; latter has max length of 2^32
 
@@ -43,7 +48,3 @@ En- & De- coding between CWasm 1.0 AST & Wasm's binary format
 [wasm_notationsScript.sml](wasm_notationsScript.sml):
 Notations for cake's Wasm 1.0 AST
 Separated from wasmLangScript for ergonomics/build efficency
-
-[wasm_parseScript.sml](wasm_parseScript.sml):
-To deprecate/delete
-WASM parser -- supports part of WASM text format
